common/Memory.v
@@ -4275,7 +4275,7 @@ Variable P: block -> Z -> Prop.
 
 Record unchanged_on (m_before m_after: mem) : Prop := mk_unchanged_on {
   unchanged_on_nextblock:
-    Ple (nextblock m_before) (nextblock m_after);
+    Block.le (nextblock m_before) (nextblock m_after);
   unchanged_on_perm:
     forall b ofs k p,
     P b ofs -> valid_block m_before b ->
@@ -4290,14 +4290,15 @@ Record unchanged_on (m_before m_after: mem) : Prop := mk_unchanged_on {
 Lemma unchanged_on_refl:
   forall m, unchanged_on m m.
 Proof.
-  intros; constructor. apply Ple_refl. tauto. tauto.
+  intros; constructor. apply Block.le_refl. tauto. tauto.
 Qed.
 
 Lemma valid_block_unchanged_on:
   forall m m' b,
   unchanged_on m m' -> valid_block m b -> valid_block m' b.
 Proof.
-  unfold valid_block; intros. apply unchanged_on_nextblock in H. xomega.
+  unfold valid_block; intros. apply unchanged_on_nextblock in H.
+  eapply Block.lt_le_trans; eauto.
 Qed.
 
 Lemma perm_unchanged_on:
@@ -4320,7 +4321,7 @@ Lemma unchanged_on_trans:
   forall m1 m2 m3, unchanged_on m1 m2 -> unchanged_on m2 m3 -> unchanged_on m1 m3.
 Proof.
   intros; constructor.
-- apply Ple_trans with (nextblock m2); apply unchanged_on_nextblock; auto.
+- apply Block.le_trans with (nextblock m2); apply unchanged_on_nextblock; auto.
 - intros. transitivity (perm m2 b ofs k p); apply unchanged_on_perm; auto.
   eapply valid_block_unchanged_on; eauto.
 - intros. transitivity (ZMap.get ofs (mem_contents m2)#b); apply unchanged_on_contents; auto.
@@ -4394,7 +4395,7 @@ Lemma store_unchanged_on:
   unchanged_on m m'.
 Proof.
   intros; constructor; intros.
-- rewrite (nextblock_store _ _ _ _ _ _ H). apply Ple_refl.
+- rewrite (nextblock_store _ _ _ _ _ _ H). apply Block.le_refl.
 - split; intros; eauto with mem.
 - erewrite store_mem_contents; eauto. rewrite BMap.gsspec.
   destruct (BMap.elt_eq b0 b); auto. subst b0. apply setN_outside.
@@ -4411,7 +4412,7 @@ Lemma storebytes_unchanged_on:
   unchanged_on m m'.
 Proof.
   intros; constructor; intros.
-- rewrite (nextblock_storebytes _ _ _ _ _ H). apply Ple_refl.
+- rewrite (nextblock_storebytes _ _ _ _ _ H). apply Block.le_refl.
 - split; intros. eapply perm_storebytes_1; eauto. eapply perm_storebytes_2; eauto.
 - erewrite storebytes_mem_contents; eauto. rewrite BMap.gsspec.
   destruct (BMap.elt_eq b0 b); auto. subst b0. apply setN_outside.
@@ -4426,7 +4427,7 @@ Lemma alloc_unchanged_on:
   unchanged_on m m'.
 Proof.
   intros; constructor; intros.
-- rewrite (nextblock_alloc _ _ _ _ _ H). apply Ple_succ.
+- rewrite (nextblock_alloc _ _ _ _ _ H). apply Block.lt_le, Block.lt_succ.
 - split; intros.
   eapply perm_alloc_1; eauto.
   eapply perm_alloc_4; eauto.
@@ -4442,7 +4443,7 @@ Lemma free_unchanged_on:
   unchanged_on m m'.
 Proof.
   intros; constructor; intros.
-- rewrite (nextblock_free _ _ _ _ _ H). apply Ple_refl.
+- rewrite (nextblock_free _ _ _ _ _ H). apply Block.le_refl.
 - split; intros.
   eapply perm_free_1; eauto.
   destruct (eq_block b0 b); auto. destruct (zlt ofs lo); auto. destruct (zle hi ofs); auto.
@@ -4459,7 +4460,7 @@ Lemma drop_perm_unchanged_on:
   unchanged_on m m'.
 Proof.
   intros; constructor; intros.
-- rewrite (nextblock_drop _ _ _ _ _ _ H). apply Ple_refl.
+- rewrite (nextblock_drop _ _ _ _ _ _ H). apply Block.le_refl.
 - split; intros. eapply perm_drop_3; eauto.
   destruct (eq_block b0 b); auto.
   subst b0.
